
\begin{problem}{3}
  假设 $T\in \Hom(\F^n,\F^m)$.  
  证明存在$A_{j,k}\in\F$ ，其中 $j=1,\dots,m$
   $k=1,\dots,n$， 使得
  \begin{equation*}
  T(x_1,\dots,x_n) = (A_{1,1}x_1 + \dots + A_{1,n}x_n,\dots, A_{m,1}x_1 + \dots + A_{m,n}x_n)
  \end{equation*}
  对于每一个 $(x_1,\dots,x_n)\in\F^n$都成立.
\end{problem}
  %------------------------------------------------
\begin{proof}[Proof]
  对于任意的 $x\in\F^n$，我们可以写 
  \begin{equation*}
    x = x_1 e_1 + \dots + x_n e_n,
  \end{equation*}
  其中 $e_1,\dots,e_n$ 是 $\F^n$ 的标准基.  
  因为 $T$ 是线性的，我们有
  \begin{equation*}
    Tx = T(x_1 e_1 + \dots +x_n e_n) = x_1 Te_1 + \dots + x_n Te_n.
  \end{equation*}
  现在对于 $Te_k\in\F^m$, 其中 $k=1,\dots, n$, 都存在 
  $A_{1,k},\dots, A_{m,k}\in\F$ 使得
  \begin{align*}
    Te_k &= A_{1,k}e_1 + \dots + A_{m,k}e_m\\
        &= \left(A_{1,k}, \dots, A_{m,k}\right)
  \end{align*}
  因此
  \begin{equation*}
    x_kTe_k = \left(A_{1,k}x_k, \dots, A_{m,k}x_k\right).
  \end{equation*}
  所以我们有
  \begin{align*}
    Tx &= \sum_{k = 1}^n \left(A_{1,k}x_k, \dots, A_{m,k}x_k\right)\\
       &= \left(\sum_{k = 1}^nA_{1,k}x_k, \dots, \sum_{k = 1}^nA_{m,k}x_k \right),
  \end{align*}
  就证得存在$A_{j,k}\in\F$ ，其中 $j=1,\dots,m$ 并且 $k=1,\dots,n$ 使得等式成立.
\end{proof}
